FSM/ProductMachine.thy
@@ -1,0 +1,626 @@
+theory ProductMachine
+imports FSM
+
+begin
+
+
+subsection \<open>Product Machine\<close>
+
+fun product_transitions :: "('state1, 'b) FSM_scheme \<Rightarrow> ('state2, 'c) FSM_scheme \<Rightarrow> ('state1 \<times> 'state2) Transition list" where
+  "product_transitions A B = map (\<lambda> (t1,t2). ((t_source t1, t_source t2),t_input t1,t_output t1,(t_target t1,t_target t2))) (filter (\<lambda> (t1,t2) . t_input t1 = t_input t2 \<and> t_output t1 = t_output t2) (cartesian_product_list (wf_transitions A) (wf_transitions B)))"
+
+
+value "product_transitions M_ex M_ex'"
+
+
+
+
+
+    
+
+lemma product_transitions_alt1 : "set (product_transitions A B) = {((t_source t1, t_source t2),t_input t1,t_output t1,(t_target t1, t_target t2)) | t1 t2 . (t1,t2) \<in> set (cartesian_product_list (wf_transitions A) (wf_transitions B)) \<and> t_input t1 = t_input t2 \<and> t_output t1 = t_output t2}"
+proof 
+  show "set (product_transitions A B) \<subseteq> {((t_source t1, t_source t2),t_input t1,t_output t1,(t_target t1, t_target t2)) | t1 t2 . (t1,t2) \<in> set (cartesian_product_list (wf_transitions A) (wf_transitions B)) \<and> t_input t1 = t_input t2 \<and> t_output t1 = t_output t2}"
+  proof 
+    fix x assume "x \<in> set (product_transitions A B)"
+    then obtain t1 t2 where "x = ((t_source t1, t_source t2),t_input t1,t_output t1,(t_target t1,t_target t2))"
+                        and "t_input t1 = t_input t2 \<and> t_output t1 = t_output t2"
+                        and "(t1,t2) \<in> set (cartesian_product_list (wf_transitions A) (wf_transitions B))"
+      by force
+    then show "x \<in> {((t_source t1, t_source t2),t_input t1,t_output t1,(t_target t1, t_target t2)) | t1 t2 . (t1,t2) \<in> set (cartesian_product_list (wf_transitions A) (wf_transitions B)) \<and> t_input t1 = t_input t2 \<and> t_output t1 = t_output t2}" by blast
+  qed
+
+  show "{((t_source t1, t_source t2),t_input t1,t_output t1,(t_target t1, t_target t2)) | t1 t2 . (t1,t2) \<in> set (cartesian_product_list (wf_transitions A) (wf_transitions B)) \<and> t_input t1 = t_input t2 \<and> t_output t1 = t_output t2} \<subseteq> set (product_transitions A B)"
+    by force
+qed
+
+lemma product_transitions_alt2 : "set (product_transitions A B) = {((t_source t1, t_source t2),t_input t1,t_output t1,(t_target t1, t_target t2)) | t1 t2 . t1 \<in> set (wf_transitions A) \<and> t2 \<in> set (wf_transitions B) \<and> t_input t1 = t_input t2 \<and> t_output t1 = t_output t2}"
+(is "?P = ?A2")
+proof -
+  have "?P = {((t_source t1, t_source t2),t_input t1,t_output t1,(t_target t1, t_target t2)) | t1 t2 . (t1,t2) \<in> set (cartesian_product_list (wf_transitions A) (wf_transitions B)) \<and> t_input t1 = t_input t2 \<and> t_output t1 = t_output t2}"
+    using product_transitions_alt1 by assumption
+  also have "... = ?A2" by force
+  finally show ?thesis by auto
+qed
+
+lemma product_transitions_alt3 : "set (product_transitions A B) = {((q1,q2),x,y,(q1',q2')) | q1 q2 x y q1' q2' . (q1,x,y,q1') \<in> set (wf_transitions A) \<and> (q2,x,y,q2') \<in> set (wf_transitions B)}"
+(is "?P = ?A3")
+proof -
+  have "?P = {((t_source t1, t_source t2),t_input t1,t_output t1,(t_target t1, t_target t2)) | t1 t2 . t1 \<in> set (wf_transitions A) \<and> t2 \<in> set (wf_transitions B) \<and> t_input t1 = t_input t2 \<and> t_output t1 = t_output t2}"
+    using product_transitions_alt2 by assumption
+  also have "... = ?A3" by force
+  finally show ?thesis by simp
+qed
+
+
+fun product :: "('state1, 'b) FSM_scheme \<Rightarrow> ('state2, 'c) FSM_scheme \<Rightarrow> (('state1 \<times> 'state2), 'b) FSM_scheme" where
+  "product A B =
+  \<lparr>
+    initial = (initial A, initial B),
+    inputs = (inputs A) @ (inputs B),
+    outputs = (outputs A) @ (outputs B),
+    transitions = product_transitions A B,
+    \<dots> = FSM.more A    
+  \<rparr>"
+
+
+value "product M_ex M_ex'"
+
+abbreviation(input) "left_path p \<equiv> map (\<lambda>t. (fst (t_source t), t_input t, t_output t, fst (t_target t))) p"
+abbreviation(input) "right_path p \<equiv> map (\<lambda>t. (snd (t_source t), t_input t, t_output t, snd (t_target t))) p"
+abbreviation(input) "zip_path p1 p2 \<equiv> (map (\<lambda> t . ((t_source (fst t), t_source (snd t)), t_input (fst t), t_output (fst t), (t_target (fst t), t_target (snd t)))) (zip p1 p2))"
+
+
+lemma product_simps[simp]:
+  "initial (product A B) = (initial A, initial B)"  
+  "inputs (product A B) = inputs A @ inputs B"
+  "outputs (product A B) = outputs A @ outputs B"
+  "transitions (product A B) = product_transitions A B"
+unfolding product_def by simp+
+
+
+
+
+lemma product_transitions_io_valid :
+  "set (product_transitions A B) = hIO (product A B)"
+proof -
+  have "\<And> t . t \<in> set (product_transitions A B) \<Longrightarrow> t \<in> hIO (product A B)"
+  proof -
+    fix t assume *: "t \<in> set (product_transitions A B)"
+    then obtain t1 t2 where "t = ((t_source t1, t_source t2), t_input t1, t_output t1, t_target t1, t_target t2)"
+                        and "t1 \<in> h A \<and> t2 \<in> h B \<and> t_input t1 = t_input t2 \<and> t_output t1 = t_output t2"
+      using product_transitions_alt2[of A B] by blast
+    then have "is_io_valid_transition (product A B) t"
+      by auto
+    then show "t \<in> hIO (product A B)" using *
+      by (metis io_valid_transition_simp product_simps(4))
+  qed
+  moreover have "\<And> t . t \<in> hIO (product A B) \<Longrightarrow>  t \<in> set (product_transitions A B)"
+    by (metis io_valid_transition_simp product_simps(4))
+  ultimately show ?thesis by blast
+qed
+  
+
+lemma product_transition_hIO :
+  "((q1,q2),x,y,(q1',q2')) \<in> hIO (product A B) \<longleftrightarrow> (q1,x,y,q1') \<in> h A \<and> (q2,x,y,q2') \<in> h B"
+  using product_transitions_io_valid[of A B] product_transitions_alt3[of A B] by blast
+
+
+
+
+
+lemma zip_path_last : "length xs = length ys \<Longrightarrow> (zip_path (xs @ [x]) (ys @ [y])) = (zip_path xs ys)@(zip_path [x] [y])"
+  by (induction xs ys rule: list_induct2; simp)
+
+lemma product_path_from_paths :
+  assumes "path A (initial A) p1"
+      and "path B (initial B) p2"
+      and "p_io p1 = p_io p2"
+    shows "path (product A B) (initial (product A B)) (zip_path p1 p2)"
+      and "target (zip_path p1 p2) (initial (product A B)) = (target p1 (initial A), target p2 (initial B))"
+proof -
+  have "initial (product A B) = (initial A, initial B)" by auto
+  then have "(initial A, initial B) \<in> nodes (product A B)"
+    by (metis nodes.initial) 
+
+  have "length p1 = length p2" using assms(3)
+    using map_eq_imp_length_eq by blast 
+  then have c: "path (product A B) (initial (product A B)) (zip_path p1 p2) \<and> target (zip_path p1 p2) (initial (product A B)) = (target p1 (initial A), target p2 (initial B))"
+    using assms proof (induction p1 p2 rule: rev_induct2)
+    case Nil
+    
+    then have "path (product A B) (initial (product A B)) (zip_path [] [])" 
+      using \<open>initial (product A B) = (initial A, initial B)\<close> \<open>(initial A, initial B) \<in> nodes (product A B)\<close>
+      by (metis Nil_is_map_conv path.nil zip_Nil)
+    moreover have "target (zip_path [] []) (initial (product A B)) = (target [] (initial A), target [] (initial B))"
+      using \<open>initial (product A B) = (initial A, initial B)\<close> by auto
+    ultimately show ?case by fast
+  next
+    case (snoc x xs y ys)
+    
+    have "path A (initial A) xs" using snoc.prems(1) by auto
+    moreover have "path B (initial B) ys" using snoc.prems(2) by auto
+    moreover have "p_io xs = p_io ys" using snoc.prems(3) by auto
+    ultimately have *:"path (product A B) (initial (product A B)) (zip_path xs ys)" 
+                and **:"target (zip_path xs ys) (initial (product A B)) = (target xs (initial A), target ys (initial B))" 
+      using snoc.IH by blast+
+    then have "(target xs (initial A), target ys (initial B)) \<in> nodes (product A B)"
+      by (metis (no_types, lifting) path_target_is_node)
+    then have "(t_source x, t_source y) \<in> nodes (product A B)"
+      using snoc.prems(1-2)  by (metis path_consIO_elim path_suffix) 
+
+    have "x \<in> h A" using snoc.prems(1) by auto
+    moreover have "y \<in> h B" using snoc.prems(2) by auto
+    moreover have "t_input x = t_input y" using snoc.prems(3) by auto
+    moreover have "t_output x = t_output y" using snoc.prems(3) by auto
+    ultimately have "((t_source x, t_source y), t_input x, t_output x, (t_target x, t_target y)) \<in> hIO (product A B)"
+    proof -
+      have f1: "{((t_source p, t_source pa), t_input p, t_output p, t_target p, t_target pa) | p pa. p \<in> set (wf_transitions A) \<and> pa \<in> set (wf_transitions B) \<and> t_input p = t_input pa \<and> t_output p = t_output pa} = set (io_valid_transitions (product A B))"
+        using product_transitions_alt2[of A B] product_transitions_io_valid by blast
+      have "\<exists>p pa. ((t_source x, t_source y), t_input x, t_output x, t_target x, t_target y) = ((t_source p, t_source pa), t_input p, t_output p, t_target p, t_target pa) \<and> p \<in> set (wf_transitions A) \<and> pa \<in> set (wf_transitions B) \<and> t_input p = t_input pa \<and> t_output p = t_output pa"
+        using \<open>t_input x = t_input y\<close> \<open>t_output x = t_output y\<close> \<open>x \<in> set (wf_transitions A)\<close> \<open>y \<in> set (wf_transitions B)\<close> by blast
+      then show ?thesis
+        using f1 by blast
+    qed 
+    
+    moreover have "t_source x = target xs (initial A)" using snoc.prems(1) by auto
+    moreover have "t_source y = target ys (initial B)" using snoc.prems(2) by auto
+    ultimately have "((target xs (initial A), target ys (initial B)), t_input x, t_output x, (t_target x, t_target y)) \<in> h (product A B)"
+      using \<open>(t_source x, t_source y) \<in> nodes (product A B)\<close>
+      by (metis fst_conv io_valid_transition_simp wf_transition_simp)
+    then have ***: "path (product A B) (initial (product A B)) ((zip_path xs ys)@[((target xs (initial A), target ys (initial B)), t_input x, t_output x, (t_target x, t_target y))])"
+      using * **
+    proof -
+      have "\<forall>p f. p \<notin> nodes (f::('a \<times> 'c, 'b) FSM_scheme) \<or> path f p []"
+        by blast
+      then have "path (product A B) (t_source ((target xs (initial A), target ys (initial B)), t_input x, t_output x, t_target x, t_target y)) [((target xs (initial A), target ys (initial B)), t_input x, t_output x, t_target x, t_target y)]"
+        by (meson \<open>((target xs (initial A), target ys (initial B)), t_input x, t_output x, t_target x, t_target y) \<in> set (wf_transitions (product A B))\<close> consIO nodes.step wf_transition_simp)
+      then have "path (product A B) (target (map (\<lambda>p. ((t_source (fst p), t_source (snd p)), t_input (fst p), t_output (fst p), t_target (fst p), t_target (snd p))) (zip xs ys)) (initial (product A B))) [((target xs (initial A), target ys (initial B)), t_input x, t_output x, t_target x, t_target y)]"
+        by (metis (no_types) "**" fst_conv)
+      then show ?thesis
+        using "*" by blast
+    qed     
+
+    have "t_target x = target (xs@[x]) (initial A)" by auto
+    moreover have "t_target y = target (ys@[y]) (initial B)" by auto
+    ultimately have ****: "target ((zip_path xs ys)@[((target xs (initial A), target ys (initial B)), t_input x, t_output x, (t_target x, t_target y))]) (initial (product A B)) = (target (xs@[x]) (initial A), target (ys@[y]) (initial B))"
+      by fastforce
+
+
+    have "(zip_path [x] [y]) = [((target xs (initial A), target ys (initial B)), t_input x, t_output x, (t_target x, t_target y))]"
+      using \<open>t_source x = target xs (initial A)\<close> \<open>t_source y = target ys (initial B)\<close> by auto
+    moreover have "(zip_path (xs @ [x]) (ys @ [y])) = (zip_path xs ys)@(zip_path [x] [y])"
+      using zip_path_last[of xs ys x y, OF snoc.hyps]  by assumption
+    ultimately have *****:"(zip_path (xs@[x]) (ys@[y])) = (zip_path xs ys)@[((target xs (initial A), target ys (initial B)), t_input x, t_output x, (t_target x, t_target y))]"
+      by auto
+    then have "path (product A B) (initial (product A B)) (zip_path (xs@[x]) (ys@[y]))"
+      using *** by presburger 
+    moreover have "target (zip_path (xs@[x]) (ys@[y])) (initial (product A B)) = (target (xs@[x]) (initial A), target (ys@[y]) (initial B))"
+      using **** ***** by auto
+    ultimately show ?case by linarith
+  qed
+
+  from c show "path (product A B) (initial (product A B)) (zip_path p1 p2)" by auto
+  from c show "target (zip_path p1 p2) (initial (product A B)) = (target p1 (initial A), target p2 (initial B))" by auto
+qed
+
+
+lemma product_transitions_elem :
+  assumes "t \<in> set (product_transitions A B)"
+  shows "(fst (t_source t), t_input t, t_output t, fst (t_target t)) \<in> h A"
+    and "(snd (t_source t), t_input t, t_output t, snd (t_target t)) \<in> h B"
+proof -
+  obtain t1 t2 where *:   "t = ((t_source t1, t_source t2), t_input t1, t_output t1, t_target t1, t_target t2)" 
+                 and **:  "t1 \<in> h A"
+                 and ***: "t2 \<in> h B"
+                 and ****: "t_input t1 = t_input t2 \<and> t_output t1 = t_output t2"
+    using assms product_transitions_alt2[of A B] by blast
+ 
+  from * ** show "(fst (t_source t), t_input t, t_output t, fst (t_target t)) \<in> h A" by auto
+  from * *** **** show "(snd (t_source t), t_input t, t_output t, snd (t_target t)) \<in> h B" by auto
+qed
+
+
+lemma paths_from_product_path :
+  assumes "path (product A B) (initial (product A B)) p"
+  shows   "path A (initial A) (left_path p)"
+      and "path B (initial B) (right_path p)"
+      and "target (left_path p) (initial A) = fst (target p (initial (product A B)))"
+      and "target (right_path p) (initial B) = snd (target p (initial (product A B)))"
+proof -
+  have "path A (initial A) (left_path p)
+            \<and> path B (initial B) (right_path p)
+            \<and> target (left_path p) (initial A) = fst (target p (initial (product A B)))
+            \<and> target (right_path p) (initial B) = snd (target p (initial (product A B)))"
+  using assms proof (induction p rule: rev_induct)
+    case Nil
+    then show ?case by auto
+  next
+    case (snoc t p)
+    then have "path (product A B) (initial (product A B)) p" by fast
+    then have "path A (initial A) (left_path p)"
+      and "path B (initial B) (right_path p)"
+      and "target (left_path p) (initial A) = fst (target p (initial (product A B)))"
+      and "target (right_path p) (initial B) = snd (target p (initial (product A B)))" 
+      using snoc.IH  by fastforce+
+
+    then have "t_source t = (target (left_path p) (initial A), target (right_path p) (initial B))"
+      using snoc.prems by (metis (no_types, lifting) path_consIO_elim path_suffix prod.collapse) 
+
+
+    have ***: "target (left_path (p@[t])) (initial A) = fst (target (p@[t]) (initial (product A B)))"
+      by fastforce
+    have ****: "target (right_path (p@[t])) (initial B) = snd (target (p@[t]) (initial (product A B)))"
+      by fastforce
+
+    have "t \<in> h (product A B)" using snoc.prems
+      by (meson path_consIO_elim path_suffix wf_transition_simp) 
+    then have "t \<in> set (product_transitions A B)" 
+      using product_transitions_io_valid[of A B]
+      by (metis io_valid_transition_simp wf_transition_simp) 
+    
+    have "(fst (t_source t), t_input t, t_output t, fst (t_target t)) \<in> h A"
+      using product_transitions_elem[OF \<open>t \<in> set (product_transitions A B)\<close>] by simp
+    moreover have "target (left_path p) (initial A) = fst (t_source t)"
+      using \<open>t_source t = (target (left_path p) (initial A), target (right_path p) (initial B))\<close> by auto
+    ultimately have "path A (initial A) ((left_path p)@[(fst (t_source t), t_input t, t_output t, fst (t_target t))])"
+    proof -
+      have "\<forall>a f. a \<notin> nodes (f::('a, 'c) FSM_scheme) \<or> path f a []"
+        by blast
+      then have "path A (t_source (fst (t_source t), t_input t, t_output t, fst (t_target t))) [(fst (t_source t), t_input t, t_output t, fst (t_target t))]"
+        by (meson \<open>(fst (t_source t), t_input t, t_output t, fst (t_target t)) \<in> set (wf_transitions A)\<close> consIO nodes.simps wf_transition_simp)
+      then have "path A (target (map (\<lambda>p. (fst (t_source p), t_input p, t_output p, fst (t_target p))) p) (initial A)) [(fst (t_source t), t_input t, t_output t, fst (t_target t))]"
+        using \<open>target (map (\<lambda>t. (fst (t_source t), t_input t, t_output t, fst (t_target t))) p) (initial A) = fst (t_source t)\<close> by auto
+      then show ?thesis
+        using \<open>path A (initial A) (map (\<lambda>t. (fst (t_source t), t_input t, t_output t, fst (t_target t))) p)\<close> by blast
+    qed 
+    then have *: "path A (initial A) (left_path (p@[t]))" by auto
+
+    have "(snd (t_source t), t_input t, t_output t, snd (t_target t)) \<in> h B"
+      using product_transitions_elem[OF \<open>t \<in> set (product_transitions A B)\<close>] by simp
+    moreover have "target (right_path p) (initial B) = snd (t_source t)"
+      using \<open>t_source t = (target (left_path p) (initial A), target (right_path p) (initial B))\<close> by auto
+    ultimately have "path B (initial B) ((right_path p)@[(snd (t_source t), t_input t, t_output t, snd (t_target t))])"
+    proof -
+      have "\<forall>b f. b \<notin> nodes (f::('b, 'd) FSM_scheme) \<or> path f b []"
+        by blast
+      then have "path B (t_source (snd (t_source t), t_input t, t_output t, snd (t_target t))) [(snd (t_source t), t_input t, t_output t, snd (t_target t))]"
+        by (meson \<open>(snd (t_source t), t_input t, t_output t, snd (t_target t)) \<in> set (wf_transitions B)\<close> consIO nodes.simps wf_transition_simp)
+      then have "path B (target (map (\<lambda>p. (snd (t_source p), t_input p, t_output p, snd (t_target p))) p) (initial B)) [(snd (t_source t), t_input t, t_output t, snd (t_target t))]"
+        using \<open>target (map (\<lambda>t. (snd (t_source t), t_input t, t_output t, snd (t_target t))) p) (initial B) = snd (t_source t)\<close> by auto
+      then show ?thesis
+        using \<open>path B (initial B) (map (\<lambda>t. (snd (t_source t), t_input t, t_output t, snd (t_target t))) p)\<close> by blast
+    qed
+    then have **: "path B (initial B) (right_path (p@[t]))" by auto
+
+
+    show ?case using * ** *** **** by blast
+  qed
+
+  then show "path A (initial A) (left_path p)"
+      and "path B (initial B) (right_path p)"
+      and "target (left_path p) (initial A) = fst (target p (initial (product A B)))"
+      and "target (right_path p) (initial B) = snd (target p (initial (product A B)))" by linarith+
+qed
+
+  
+
+
+
+lemma product_transition :
+  "((q1,q2),x,y,(q1',q2')) \<in> h (product A B) \<longleftrightarrow> (q1,x,y,q1') \<in> h A \<and> (q2,x,y,q2') \<in> h B \<and> (\<exists> p1 p2 . path A (initial A) p1 \<and> path B (initial B) p2 \<and> target p1 (initial A) = q1 \<and> target p2 (initial B) = q2 \<and> p_io p1 = p_io p2)"
+proof 
+  show "((q1,q2),x,y,(q1',q2')) \<in> h (product A B) \<Longrightarrow> (q1,x,y,q1') \<in> h A \<and> (q2,x,y,q2') \<in> h B \<and> (\<exists> p1 p2 . path A (initial A) p1 \<and> path B (initial B) p2 \<and> target p1 (initial A) = q1 \<and> target p2 (initial B) = q2 \<and> p_io p1 = p_io p2)"
+  proof -
+    assume "((q1,q2),x,y,(q1',q2')) \<in> h (product A B)"
+    then have "(q1,q2) \<in> nodes (product A B)"
+      by (metis fst_conv wf_transition_simp) 
+    then obtain p where "path (product A B) (initial (product A B)) p" and "target p (initial (product A B)) = (q1,q2)"
+      by (metis path_to_node)
+
+    have "path A (initial A) (left_path p) \<and> path B (initial B) (right_path p) \<and> target (left_path p) (initial A) = q1 \<and> target (right_path p) (initial B) = q2"
+      using paths_from_product_path[OF \<open>path (product A B) (initial (product A B)) p\<close>] \<open>target p (initial (product A B)) = (q1,q2)\<close> by auto
+    moreover have "p_io (left_path p) = p_io (right_path p)" by auto
+    ultimately have "(\<exists> p1 p2 . path A (initial A) p1 \<and> path B (initial B) p2 \<and> target p1 (initial A) = q1 \<and> target p2 (initial B) = q2 \<and> p_io p1 = p_io p2)"
+      by blast
+    moreover have "(q1,x,y,q1') \<in> h A \<and> (q2,x,y,q2') \<in> h B"
+      using \<open>((q1,q2),x,y,(q1',q2')) \<in> h (product A B)\<close>
+      by (metis product_simps(4) product_transition_hIO product_transitions_io_valid wf_transition_simp)
+    ultimately show ?thesis by simp
+  qed
+
+  show "(q1,x,y,q1') \<in> h A \<and> (q2,x,y,q2') \<in> h B \<and> (\<exists> p1 p2 . path A (initial A) p1 \<and> path B (initial B) p2 \<and> target p1 (initial A) = q1 \<and> target p2 (initial B) = q2 \<and> p_io p1 = p_io p2) \<Longrightarrow> ((q1,q2),x,y,(q1',q2')) \<in> h (product A B)"
+  proof -
+    assume assm: "(q1,x,y,q1') \<in> h A \<and> (q2,x,y,q2') \<in> h B \<and> (\<exists> p1 p2 . path A (initial A) p1 \<and> path B (initial B) p2 \<and> target p1 (initial A) = q1 \<and> target p2 (initial B) = q2 \<and> p_io p1 = p_io p2)"
+    then obtain p1 p2 where pr1: "path A (initial A) p1" 
+                        and pr2: "path B (initial B) p2" 
+                        and pr3: "target p1 (initial A) = q1" 
+                        and pr4: "target p2 (initial B) = q2" 
+                        and pr5: "p_io p1 = p_io p2"
+      by blast
+
+    have "(q1,x,y,q1') \<in> h A" and "(q2,x,y,q2') \<in> h B"
+      using assm by auto
+
+    have "initial (product A B) \<in> nodes (product A B)"
+      by blast 
+    moreover have "path (product A B) (initial (product A B)) (zip_path p1 p2)"
+      using product_path_from_paths(1)[OF pr1 pr2 pr5] by assumption
+    moreover have "target (zip_path p1 p2) (initial (product A B)) = (q1,q2)"
+      using product_path_from_paths(2)[OF pr1 pr2 pr5] pr3 pr4 by fast
+    ultimately have "(q1,q2) \<in> nodes (product A B)" 
+      using nodes_path[of "product A B" "initial (product A B)" "zip_path p1 p2"] by metis
+    then have "t_source ((q1,q2),x,y,(q1',q2')) \<in> nodes (product A B)"
+      by auto
+
+    moreover have "((q1,q2),x,y,(q1',q2')) \<in> hIO (product A B)"
+      using product_transitions_alt3[of A B] \<open>(q1,x,y,q1') \<in> h A\<close> \<open>(q2,x,y,q2') \<in> h B\<close> by force
+    ultimately show "((q1,q2),x,y,(q1',q2')) \<in> h (product A B)" 
+      using hIO_alt_def[of "product A B"] h_alt_def[of "product A B"] by blast
+  qed
+qed
+
+
+    
+      
+      
+  
+
+
+
+lemma product_node_from_path :
+  "(q1,q2) \<in> nodes (product A B) \<longleftrightarrow> (\<exists> p1 p2 . path A (initial A) p1 \<and> path B (initial B) p2 \<and> target p1 (initial A) = q1 \<and> target p2 (initial B) = q2 \<and> p_io p1 = p_io p2)"
+proof 
+  show "(q1,q2) \<in> nodes (product A B) \<Longrightarrow> (\<exists> p1 p2 . path A (initial A) p1 \<and> path B (initial B) p2 \<and> target p1 (initial A) = q1 \<and> target p2 (initial B) = q2 \<and> p_io p1 = p_io p2)"
+  proof -
+    assume "(q1,q2) \<in> nodes (product A B)"
+    then obtain p where "path (product A B) (initial (product A B)) p" and "target p (initial (product A B)) = (q1,q2)"
+      by (metis path_to_node) 
+    then have "path A (initial A) (left_path p) \<and> path B (initial B) (right_path p) \<and> target (left_path p) (initial A) = q1 \<and> target (right_path p) (initial B) = q2 \<and> p_io (left_path p) = p_io (right_path p)"
+      using paths_from_product_path[OF \<open>path (product A B) (initial (product A B)) p\<close>] by simp
+    then show "(\<exists> p1 p2 . path A (initial A) p1 \<and> path B (initial B) p2 \<and> target p1 (initial A) = q1 \<and> target p2 (initial B) = q2 \<and> p_io p1 = p_io p2)"
+      by blast
+  qed
+
+  show "(\<exists> p1 p2 . path A (initial A) p1 \<and> path B (initial B) p2 \<and> target p1 (initial A) = q1 \<and> target p2 (initial B) = q2 \<and> p_io p1 = p_io p2) \<Longrightarrow> (q1,q2) \<in> nodes (product A B)"
+  proof -
+    assume "(\<exists> p1 p2 . path A (initial A) p1 \<and> path B (initial B) p2 \<and> target p1 (initial A) = q1 \<and> target p2 (initial B) = q2 \<and> p_io p1 = p_io p2)"
+    then obtain p1 p2 where *: "path A (initial A) p1 \<and> path B (initial B) p2 \<and> target p1 (initial A) = q1 \<and> target p2 (initial B) = q2 \<and> p_io p1 = p_io p2"
+      by blast
+
+    have "initial (product A B) \<in> nodes (product A B)"
+      by blast 
+    moreover have "path (product A B) (initial (product A B)) (zip_path p1 p2)"
+      using product_path_from_paths(1)[of A p1 B p2] * by metis
+    moreover have "target (zip_path p1 p2) (initial (product A B)) = (q1,q2)"
+      using product_path_from_paths(2)[of A p1 B p2] * by metis
+    ultimately show "(q1,q2) \<in> nodes (product A B)" 
+      using nodes_path[of "product A B" "initial (product A B)" "zip_path p1 p2"] by metis
+  qed
+qed
+
+
+lemma left_path_zip : "length p1 = length p2 \<Longrightarrow> left_path (zip_path p1 p2) = p1" 
+  by (induction p1 p2 rule: list_induct2; simp)
+
+lemma right_path_zip : "length p1 = length p2 \<Longrightarrow> p_io p1 = p_io p2 \<Longrightarrow> right_path (zip_path p1 p2) = p2" 
+  by (induction p1 p2 rule: list_induct2; simp)
+
+lemma zip_path_append_left_right : "length p1 = length p2 \<Longrightarrow> zip_path (p1@(left_path p)) (p2@(right_path p)) = (zip_path p1 p2)@p"
+proof (induction p1 p2 rule: list_induct2)
+  case Nil
+  then show ?case by (induction p; simp)
+next
+  case (Cons x xs y ys)
+  then show ?case by simp
+qed
+  
+    
+      
+
+lemma product_path:
+  "path (product A B) (q1,q2) p \<longleftrightarrow> (path A q1 (left_path p) \<and> path B q2 (right_path p) \<and> (\<exists> p1 p2 . path A (initial A) p1 \<and> path B (initial B) p2 \<and> target p1 (initial A) = q1 \<and> target p2 (initial B) = q2 \<and> p_io p1 = p_io p2))"
+proof 
+  show "path (product A B) (q1,q2) p \<Longrightarrow> (path A q1 (left_path p) \<and> path B q2 (right_path p) \<and> (\<exists> p1 p2 . path A (initial A) p1 \<and> path B (initial B) p2 \<and> target p1 (initial A) = q1 \<and> target p2 (initial B) = q2 \<and> p_io p1 = p_io p2))"
+  proof -
+    assume "path (product A B) (q1,q2) p"
+    then have "(q1,q2) \<in> nodes (product A B)"
+      by (meson path_begin_node) 
+    then have ex12: "(\<exists> p1 p2 . path A (initial A) p1 \<and> path B (initial B) p2 \<and> target p1 (initial A) = q1 \<and> target p2 (initial B) = q2 \<and> p_io p1 = p_io p2)"
+      using product_node_from_path[of q1 q2 A B] by blast
+    then obtain p1 p2 where *: "path A (initial A) p1 \<and> path B (initial B) p2 \<and> target p1 (initial A) = q1 \<and> target p2 (initial B) = q2 \<and> p_io p1 = p_io p2"
+      by blast
+    then have "path (product A B) (initial (product A B)) (zip_path p1 p2)" 
+      using product_path_from_paths(1)[of A p1 B p2] by metis
+
+    have "path A (initial A) p1" and "path B (initial B) p2" and "target p1 (initial A) = q1" and "target p2 (initial B) = q2" and "p_io p1 = p_io p2"
+      using * by linarith+
+
+    have "target (zip_path p1 p2) (initial (product A B)) = (q1,q2)"
+      using product_path_from_paths(2)[of A p1 B p2] * by metis
+
+    have "path (product A B) (initial (product A B)) ((zip_path p1 p2) @ p)" 
+      using path_append[OF \<open>path (product A B) (initial (product A B)) (zip_path p1 p2)\<close>, of p]
+            \<open>target (zip_path p1 p2) (initial (product A B)) = (q1,q2)\<close>
+            \<open>path (product A B) (q1,q2) p\<close> by metis
+
+    have "path A (initial A) (left_path ((zip_path p1 p2) @ p))"
+      and "path B (initial B) (right_path ((zip_path p1 p2) @ p))"
+      and "target (left_path ((zip_path p1 p2) @ p)) (initial A) = fst (target ((zip_path p1 p2) @ p) (initial (product A B)))"
+      and "target (right_path ((zip_path p1 p2) @ p)) (initial B) = snd (target ((zip_path p1 p2) @ p) (initial (product A B)))"
+      using paths_from_product_path[OF \<open>path (product A B) (initial (product A B)) ((zip_path p1 p2) @ p)\<close>] by linarith+
+
+    have "length p1 = length p2"
+      using \<open>p_io p1 = p_io p2\<close> map_eq_imp_length_eq by blast 
+
+    have "(left_path ((zip_path p1 p2) @ p)) = p1@(left_path p)"
+      using left_path_zip[OF \<open>length p1 = length p2\<close>] by (induction p; simp)
+    then have "path A (initial A) (p1@(left_path p))"
+      using \<open>path A (initial A) (left_path ((zip_path p1 p2) @ p))\<close> by simp
+    have lp: "path A q1 (left_path p)" 
+      using path_suffix[OF \<open>path A (initial A) (p1@(left_path p))\<close>] \<open>target p1 (initial A) = q1\<close> by simp
+
+    
+    have "(right_path ((zip_path p1 p2) @ p)) = p2@(right_path p)"
+      using right_path_zip[OF \<open>length p1 = length p2\<close> \<open>p_io p1 = p_io p2\<close>] by (induction p; simp)  
+    then have "path B (initial B) (p2@(right_path p))"
+      using \<open>path B (initial B) (right_path ((zip_path p1 p2) @ p))\<close> by simp
+    have rp: "path B q2 (right_path p)" 
+      using path_suffix[OF \<open>path B (initial B) (p2@(right_path p))\<close>] \<open>target p2 (initial B) = q2\<close> by simp  
+
+    show "(path A q1 (left_path p) \<and> path B q2 (right_path p) \<and> (\<exists> p1 p2 . path A (initial A) p1 \<and> path B (initial B) p2 \<and> target p1 (initial A) = q1 \<and> target p2 (initial B) = q2 \<and> p_io p1 = p_io p2))"
+      using lp rp ex12 by simp
+  qed
+
+
+  show "(path A q1 (left_path p) \<and> path B q2 (right_path p) \<and> (\<exists> p1 p2 . path A (initial A) p1 \<and> path B (initial B) p2 \<and> target p1 (initial A) = q1 \<and> target p2 (initial B) = q2 \<and> p_io p1 = p_io p2)) \<Longrightarrow> path (product A B) (q1,q2) p"
+  proof-
+    assume "(path A q1 (left_path p) \<and> path B q2 (right_path p) \<and> (\<exists> p1 p2 . path A (initial A) p1 \<and> path B (initial B) p2 \<and> target p1 (initial A) = q1 \<and> target p2 (initial B) = q2 \<and> p_io p1 = p_io p2))"
+    then have "path A q1 (left_path p)" and "path B q2 (right_path p)" and "(\<exists> p1 p2 . path A (initial A) p1 \<and> path B (initial B) p2 \<and> target p1 (initial A) = q1 \<and> target p2 (initial B) = q2 \<and> p_io p1 = p_io p2)"
+      by auto
+    then obtain p1 p2 where *: "path A (initial A) p1" and "path B (initial B) p2" and "target p1 (initial A) = q1" and "target p2 (initial B) = q2" and "p_io p1 = p_io p2"
+      by blast 
+
+    have "path A (initial A) (p1@(left_path p))"
+      using path_append[OF \<open>path A (initial A) p1\<close>, of "left_path p"] \<open>target p1 (initial A) = q1\<close> \<open>path A q1 (left_path p)\<close> by metis
+    have "path B (initial B) (p2@(right_path p))"
+      using path_append[OF \<open>path B (initial B) p2\<close>, of "right_path p"] \<open>target p2 (initial B) = q2\<close> \<open>path B q2 (right_path p)\<close> by metis
+    have "p_io (p1@(left_path p)) = p_io (p2@(right_path p))"
+      using \<open>p_io p1 = p_io p2\<close> by (induction p; simp)
+    
+    have "path (product A B) (initial (product A B)) ((zip_path p1 p2)@p)"
+      using product_path_from_paths(1)[OF \<open>path A (initial A) (p1@(left_path p))\<close> \<open>path B (initial B) (p2@(right_path p))\<close> \<open>p_io (p1@(left_path p)) = p_io (p2@(right_path p))\<close>]
+            zip_path_append_left_right[of p1 p2 p]
+      by (metis (no_types, lifting) \<open>p_io p1 = p_io p2\<close> map_eq_imp_length_eq) 
+
+    have "path (product A B) (initial (product A B)) (zip_path p1 p2)"
+      using product_path_from_paths(1)[OF \<open>path A (initial A) p1\<close> \<open>path B (initial B) p2\<close> \<open>p_io p1 = p_io p2\<close>] by metis
+    moreover have "target (zip_path p1 p2) (initial (product A B)) = (q1,q2)"
+      using product_path_from_paths(2)[OF \<open>path A (initial A) p1\<close> \<open>path B (initial B) p2\<close> \<open>p_io p1 = p_io p2\<close>] \<open>target p1 (initial A) = q1\<close> \<open>target p2 (initial B) = q2\<close> by metis
+    
+    
+    ultimately show "path (product A B) (q1,q2) p"
+      using path_suffix[OF \<open>path (product A B) (initial (product A B)) ((zip_path p1 p2)@p)\<close>]
+      by presburger 
+  qed
+qed
+    
+      
+
+
+
+
+
+
+
+
+
+
+
+
+lemma product_path_rev:
+  assumes "p_io p1 = p_io p2"
+  shows "path (product A B) (q1,q2) (zip_path p1 p2)
+          \<longleftrightarrow> (path A q1 p1 \<and> path B q2 p2 \<and> (\<exists> p1 p2 . path A (initial A) p1 \<and> path B (initial B) p2 \<and> target p1 (initial A) = q1 \<and> target p2 (initial B) = q2 \<and> p_io p1 = p_io p2))"
+proof -
+  have "length p1 = length p2" using assms
+    using map_eq_imp_length_eq by blast 
+  then have "(map (\<lambda> t . (fst (t_source t), t_input t, t_output t, fst (t_target t))) (map (\<lambda> t . ((t_source (fst t), t_source (snd t)), t_input (fst t), t_output (fst t), (t_target (fst t), t_target (snd t)))) (zip p1 p2))) = p1"
+    by (induction p1 p2 arbitrary: q1 q2 rule: list_induct2; auto)
+
+  moreover have "(map (\<lambda> t . (snd (t_source t), t_input t, t_output t, snd (t_target t))) (map (\<lambda> t . ((t_source (fst t), t_source (snd t)), t_input (fst t), t_output (fst t), (t_target (fst t), t_target (snd t)))) (zip p1 p2))) = p2"
+    using \<open>length p1 = length p2\<close> assms by (induction p1 p2 arbitrary: q1 q2 rule: list_induct2; auto)
+
+  ultimately show ?thesis using product_path[of A B q1 q2 "(map (\<lambda> t . ((t_source (fst t), t_source (snd t)), t_input (fst t), t_output (fst t), (t_target (fst t), t_target (snd t)))) (zip p1 p2))"]
+    by auto
+qed
+    
+    
+
+
+
+
+
+
+lemma product_language_state : 
+  assumes "(\<exists> p1 p2 . path A (initial A) p1 \<and> path B (initial B) p2 \<and> target p1 (initial A) = q1 \<and> target p2 (initial B) = q2 \<and> p_io p1 = p_io p2)"
+  shows "LS (product A B) (q1,q2) = LS A q1 \<inter> LS B q2"
+proof 
+  show "LS (product A B) (q1, q2) \<subseteq> LS A q1 \<inter> LS B q2"
+  proof 
+    fix io assume "io \<in> LS (product A B) (q1, q2)"
+    then obtain p where "io = p_io p" 
+                    and "path (product A B) (q1,q2) p"
+      by auto
+    then obtain p1 p2 where "path A q1 p1" 
+                        and "path B q2 p2"
+                        and "io = p_io p1" 
+                        and "io = p_io p2"
+      using product_path[of A B q1 q2 p] by fastforce
+    then show "io \<in> LS A q1 \<inter> LS B q2" 
+      unfolding LS.simps by blast
+  qed
+
+  show "LS A q1 \<inter> LS B q2 \<subseteq> LS (product A B) (q1, q2)"
+  proof
+    fix io assume "io \<in> LS A q1 \<inter> LS B q2"
+    then obtain p1 p2 where "path A q1 p1" 
+                        and "path B q2 p2"
+                        and "io = p_io p1" 
+                        and "io = p_io p2"
+                        and "p_io p1 = p_io p2"
+      by auto
+
+    let ?p = "zip_path p1 p2"
+    
+    
+    have "length p1 = length p2"
+      using \<open>p_io p1 = p_io p2\<close> map_eq_imp_length_eq by blast 
+    moreover have "p_io ?p = p_io (map fst (zip p1 p2))" by auto
+    ultimately have "p_io ?p = p_io p1" by auto
+
+    then have "p_io ?p = io" 
+      using \<open>io = p_io p1\<close> by auto
+    moreover have "path (product A B) (q1, q2) ?p"
+      using product_path_rev[OF \<open>p_io p1 = p_io p2\<close>, of A B q1 q2] \<open>path A q1 p1\<close> \<open>path B q2 p2\<close> assms by auto
+    ultimately show "io \<in> LS (product A B) (q1, q2)" 
+      unfolding LS.simps by blast
+  qed
+qed
+
+
+lemma product_language : "L (product A B) = L A \<inter> L B"
+proof -
+  have "path A (initial A) [] \<and>
+         path B (initial B) [] \<and>
+         target [] (initial A) = initial A \<and> target [] (initial B) = initial B \<and> p_io [] = p_io []" by auto
+  then have "\<exists>p1 p2.
+       path A (initial A) p1 \<and>
+       path B (initial B) p2 \<and>
+       target p1 (initial A) = initial A \<and> target p2 (initial B) = initial B \<and> p_io p1 = p_io p2" by blast
+  then show ?thesis
+    using product_language_state[of A B "initial A" "initial B"] unfolding product.simps by simp
+qed
+
+lemma product_nodes : "nodes (product A B) \<subseteq> (nodes A) \<times> (nodes B)"
+proof 
+  fix q assume "q \<in> nodes (product A B)"
+  then obtain p where "path (product A B) (initial (product A B)) p"
+                and   "q = target p (initial (product A B))" 
+    by (metis path_to_node)
+
+  let ?p1 = "left_path p"
+  let ?p2 = "right_path p"
+
+  have "path A (initial A) ?p1 \<and> path B (initial B) ?p2"
+    by (metis \<open>path (product A B) (initial (product A B)) p\<close> product_path[of A B "initial A" "initial B" p] product_simps(1))
+
+  moreover have "target p (initial (product A B)) = (target ?p1 (initial A), target ?p2 (initial B))"
+    by (induction p; force)  
+
+  ultimately show "q \<in> (nodes A) \<times> (nodes B)"
+    by (metis (no_types, lifting) SigmaI \<open>q = target p (initial (product A B))\<close> nodes_path_initial)
+qed
+
+
+end
